Experiments/SR/Data/PS/Thm.lean
@@ -1,0 +1,711 @@
+/-
+Copyright (c) 2025 The Trestle Contributors.
+Released under the Apache License v2.0; see LICENSE for full text.
+-/
+
+import Experiments.SR.Data.PS.Defs
+import Trestle.Model.Subst
+
+namespace Trestle.PS
+
+open Trestle Model Nat
+open LitVar ILit IVar LawfulLitVar
+open PropFun
+
+abbrev PSubst := (IVar → PropForm IVar)
+
+def toSubst_fun (σ : PS) : PSubst → Fin σ.size → PSV → PSubst :=
+  fun σ idx cell => (fun v =>
+    if v.index = idx.val then
+      match PSV.varValue? cell v with
+      | none => σ v
+      | some .tr => PropForm.tr
+      | some .fls => PropForm.fls
+      | some (.lit l) => if polarity l then .var (toVar l)
+                         else .neg (.var (toVar l))
+    else σ v)
+
+def toSubst (σ : PS) : PSubst :=
+  τ.assignment.foldlIdx (init := .var) (toSubst_fun τ)
+
+theorem toSubst_fun_comm (τ : PS) :
+  ∀ (σ : PSubst) (idx₁ idx₂ : Fin τ.size),
+    (toSubst_fun τ) ((toSubst_fun τ) σ idx₁ (τ.get idx₁)) idx₂ (τ.get idx₂) =
+    (toSubst_fun τ) ((toSubst_fun τ) σ idx₂ (τ.get idx₂)) idx₁ (τ.get idx₁) := by
+  intro σ idx₁ idx₂
+  unfold toSubst_fun
+  apply funext
+  intro v
+  by_cases hidx : idx₁.val = idx₂.val
+  <;> by_cases hv₁ : v.index = idx₁.val
+  <;> by_cases hv₂ : v.index = idx₂.val
+  <;> try simp [hv₁, hv₂, hidx]
+  <;> try simp [hv₁, hv₂, hidx, Ne.symm hidx]
+
+theorem toSubst_of_comm (τ : PS) {v : IVar} (hv : v.index < τ.size) :
+    ∃ σ, τ.toSubst = (toSubst_fun τ) σ ⟨v.index, hv⟩ (τ.get ⟨v.index, hv⟩) :=
+  Array.foldlIdx_of_comm τ.assignment (toSubst_fun τ) .var (toSubst_fun_comm τ) ⟨v.index, hv⟩
+
+instance : ToString PS where
+  toString τ := String.intercalate " ∧ "
+    (τ.assignment.foldl (init := []) (f := fun acc a =>
+      match a.val with
+        | .tr => s!"{a.generation}" :: acc
+        | .fls => s!"-{a.generation}" :: acc
+        | .lit l => s!"<{l}>" :: acc))
+
+@[simp]
+theorem fromMappedNat_IVarToMappedNat (v : IVar)
+    : PSV.fromMappedNat (IVarToMappedNat v) = v := by
+  have ⟨v, hv⟩ := v
+  simp [IVarToMappedNat, PSV.fromMappedNat]
+  split <;> try omega
+  rename_i n h
+  have : n % 2 = 0 := by omega
+  simp [this]
+  congr
+  omega
+
+-- CC: This proof can probably be simplified with lemmas relating `IVarToMapped` and `ILitToMapped`
+@[simp]
+theorem fromMappedNat_ILitToMappedNat (l : ILit)
+    : PSV.fromMappedNat (ILitToMappedNat l) = l := by
+  simp [PSV.fromMappedNat, ILitToMappedNat]
+  by_cases hpol : polarity l
+  <;> simp [hpol]
+  · have ⟨l, hl⟩ := l
+    split <;> try omega
+    · rename_i h
+      simp only [_root_.mul_eq_zero, Int.natAbs_eq_zero, OfNat.ofNat_ne_zero, or_false] at h
+      exact absurd h hl
+    · rename_i n h
+      simp only [succ_eq_add_one] at h
+      have : n % 2 = 0 := by omega
+      simp only [this, ↓reduceIte, mkPos, ne_eq, Int.ofNat_eq_coe, cast_add,
+        Int.ofNat_ediv, cast_ofNat, cast_one, Sum.inl.injEq]
+      congr
+      simp only [polarity, decide_eq_true_eq] at hpol
+      omega
+  · have ⟨l, hl⟩ := l
+    split <;> try omega
+    · rename_i h
+      simp only [Nat.add_eq_right, _root_.mul_eq_zero, Int.natAbs_eq_zero,
+        OfNat.ofNat_ne_zero, or_false] at h
+      exact absurd h hl
+    · rename_i n h
+      simp only [succ_eq_add_one, Nat.add_left_inj] at h
+      have : n % 2 = 1 := by omega
+      simp only [this, one_ne_zero, ↓reduceIte, mkNeg, ne_eq,
+        Int.ofNat_eq_coe, cast_add, Int.ofNat_ediv, cast_ofNat,
+        cast_one, neg_add_rev, Int.reduceNeg, Sum.inl.injEq]
+      congr
+      simp only [polarity, decide_eq_true_eq, not_lt] at hpol
+      omega
+
+/-! # negate -/
+
+-- CC: This is probably too much machinery/abstraction, but the ability to
+--     return `Nat` rather than `ILit ⊕ Bool` gives nice speedups in practice
+
+@[simp]
+theorem negateMappedNat_negateMappedNat (n : ℕ)
+    : negateMappedNat (negateMappedNat n) = n := by
+  by_cases hn : n % 2 = 0
+  <;> simp [negateMappedNat, hn]
+  · simp [succ_mod_two_eq_one_iff.mpr hn]
+  · have : (n - 1) % 2 = 0 := by omega
+    simp only [this, ↓reduceIte]
+    rw [Nat.sub_add_cancel (by omega)]
+
+@[simp]
+theorem litValue_Nat_negate (σ : PS) (l : ILit)
+    : σ.litValue_Nat (-l) = negateMappedNat (σ.litValue_Nat l) := by
+  cases hpol : polarity l <;> simp [hpol, litValue_Nat]
+
+theorem PSV.negate_eq_iff_eq_negate {p₁ p₂ : PSV}
+    : PSV.negate p₁ = p₂ ↔ p₁ = PSV.negate p₂ := by
+  cases p₁ <;> cases p₂
+  <;> simp [negate]
+  · exact neg_eq_iff_eq_neg
+
+@[simp]
+theorem PSV.negate_bool (b : Bool) : PSV.negate (.inr b) = (.inr !b) :=
+  rfl
+
+@[simp]
+theorem PSV.negate_mkPos (v : IVar)
+    : PSV.negate (.inl (mkPos v)) = (.inl (mkNeg v)) :=
+  rfl
+
+@[simp]
+theorem PSV.negate_mkNeg (v : IVar)
+    : PSV.negate (.inl (mkNeg v)) = (.inl (mkPos v)) := by
+  simp only [negate, neg_mkNeg]
+
+@[simp]
+theorem PSV.negate_neg (l : ILit)
+    : PSV.negate (.inl l) = .inl (-l) := by
+  rfl
+
+@[simp]
+theorem fromMappedNat_negateMappedNat (n : ℕ)
+    : PSV.fromMappedNat (negateMappedNat n) = PSV.negate (PSV.fromMappedNat n) := by
+  simp [negateMappedNat, PSV.fromMappedNat]
+  match n with
+  | 0 => simp only [zero_mod, ↓reduceIte, zero_add, PSV.negate_bool, Bool.not_true]
+  | 1 => simp only [mod_succ, one_ne_zero, ↓reduceIte, tsub_self, PSV.negate_bool, Bool.not_false]
+  | (n + 2) =>
+    by_cases hn : (n + 2) % 2 = 0
+    <;> simp [hn]
+    -- CC: All these omega proofs make me sad
+    · have : (n + 1) % 2 = 1 := by omega
+      simp [this]
+      have : n % 2 = 0 := by omega
+      simp [this]
+      have : (n + 1) / 2 + 1 = n / 2 + 1 := by omega
+      simp [this]
+    · have : n % 2 = 1 := by omega
+      simp [this]
+      split <;> try omega
+      rename_i hn
+      simp at hn
+      subst hn
+      rename_i n
+      simp [succ_mod_two_eq_one_iff.mp this]
+      have : (n + 1) / 2 + 1 = n / 2 + 1 := by omega
+      simp [this]
+
+@[simp]
+theorem litValue_negate (σ : PS) (l : ILit) :
+    (σ.litValue (-l)) = PSV.negate (σ.litValue l) := by
+  cases hpol : polarity l
+  <;> simp only [litValue, litValue_Nat_negate, fromMappedNat_negateMappedNat]
+
+theorem litValue_eq_varValue_pos {l : ILit} :
+    polarity l = true → ∀ (σ : PS), σ.litValue l = σ.varValue (toVar l) := by
+  intro hl σ
+  simp only [litValue, litValue_Nat, hl, ↓reduceIte, varValue]
+
+theorem litValue_eq_varValue_neg {l : ILit} :
+    polarity l = false → ∀ (σ : PS), σ.litValue l = PSV.negate (σ.varValue (toVar l)) := by
+  intro hl
+  simp only [litValue, litValue_Nat, hl, Bool.false_eq_true, ↓reduceIte,
+    fromMappedNat_negateMappedNat, varValue, implies_true]
+
+theorem litValue_eq_varValue_neg' {l : ILit} :
+    polarity l = false → ∀ (σ : PS), σ.litValue (-l) = σ.varValue (toVar l) := by
+  intro hl
+  simp only [litValue, litValue_Nat, polarity_negate, hl, Bool.not_false,
+    ↓reduceIte, toVar_negate, varValue, implies_true]
+
+theorem lt_size_of_varValue_of_not_id {σ : PS} {v : IVar} :
+    σ.varValue v ≠ (.inl (mkPos v)) → v.index < σ.size := by
+  intro hv
+  by_contra
+  rename (¬v.index < σ.size) => h_con
+  simp [varValue, varValue_Nat, h_con] at hv
+
+theorem lt_size_of_litValue_of_not_id {σ : PS} {l : ILit} :
+    σ.litValue l ≠ (.inl l) → l.index < σ.size := by
+  intro h
+  rw [← ILit.toVar_index]
+  apply lt_size_of_varValue_of_not_id
+  intro h_con
+  rcases mkPos_or_mkNeg l with (hl | hl)
+  · have hpol : polarity l = true := by rw [hl]; simp only [polarity_mkPos]
+    rw [litValue_eq_varValue_pos hpol σ, hl] at h
+    simp only [toVar_mkPos, h_con, ne_eq, not_true_eq_false] at h
+  · have hpol : polarity l = false := by rw [hl]; simp only [polarity_mkNeg]
+    rw [litValue_eq_varValue_neg hpol σ, hl] at h
+    simp [h_con] at h
+
+theorem varValue_fls_iff {σ : PS} {v : IVar} :
+    (σ.varValue v = .fls) ↔ (PropFun.bind σ.toSubst ⟦v⟧) = ⊥ := by
+  sorry
+  done
+
+theorem varValue_tr_iff {σ : PS} {v : IVar} :
+    (σ.varValue v = .tr) ↔ (PropFun.bind σ.toSubst ⟦v⟧) = ⊤ := by
+  sorry
+  done
+
+theorem varValue_lit_iff {σ : PS} {v : IVar} {l : ILit} :
+    (σ.varValue v = .lit l) ↔ (PropFun.bind σ.toSubst ⟦v⟧) = (PropFun.bind σ.toSubst l) := by
+  sorry
+  done
+
+theorem litValue_fls_iff {σ : PS} {l : ILit} :
+    (σ.litValue l = .fls) ↔ (PropFun.bind σ.toSubst l) = ⊥ := by
+  sorry
+  done
+
+theorem litValue_tr_iff {σ : PS} {l : ILit} :
+    (σ.litValue l = .tr) ↔ (PropFun.bind σ.toSubst l) = ⊤ := by
+  sorry
+  done
+
+theorem litValue_lit_iff {σ : PS} {l₁ l₂ : ILit} :
+    (σ.litValue l₁ = .lit l₂) ↔ (PropFun.bind σ.toSubst l₁) = l₂ := by
+  sorry
+  done
+
+/-! # setLit -/
+
+-- Cayden TODO: How to make setF more efficient when the value needs to be a cell?
+-- Can an efficient implementation do this linearly? Ow will run out of memory?
+-- One idea is to use a .setF' that takes a function : (Option α → α) instead of value v : α
+-- That way, if the cell exists, its value can be mapped
+
+-- This is a more efficient version
+/-
+def setLit (τ : PS) (l : ILit) : PS := { τ with
+  assignment :=
+    if hidx : l.index < τ.size then
+      τ.assignment.set ⟨l.index, hidx⟩ ((τ.get ⟨l.index, hidx⟩).setLit l τ.generation)
+    else
+      τ.assignment.setF l.index (PSCell.mkEmptyCell.setLit l τ.generation) PSCell.mkEmptyCell
+  maxGen := max τ.maxGen τ.generation
+}
+-/
+
+theorem setVar_le_maxGen (τ : PS) (i : Nat) (c : PSCell) :
+    ∀ cell ∈ (τ.assignment.setF i c PSCell.mkEmptyCell).data, cell.generation ≤ max τ.maxGen c.generation := by
+  sorry
+  done
+
+-- This is a more functional version
+/-- Set the given literal to `true` for the current generation in the PS. -/
+def setLit (τ : PS) (l : ILit) : PS := { τ with
+  assignment := τ.assignment.setF l.index (PSCell.mkEmptyCell.setLit l τ.generation) PSCell.mkEmptyCell
+  maxGen := max τ.maxGen τ.generation
+  le_maxGen := by
+    have := setVar_le_maxGen τ l.index (PSCell.mkEmptyCell.setLit l τ.generation)
+    rwa [PSCell.setLit_generation PSCell.mkEmptyCell l ↑τ.generation] at this
+}
+
+/-- Set the given literal to `true` for all generations until `gen`. -/
+def setLitUntil (τ : PS) (l : ILit) (gen : Nat) : PS := { τ with
+  assignment := τ.assignment.setF l.index (PSCell.mkEmptyCell.setLit l gen) PSCell.mkEmptyCell
+  maxGen := max τ.maxGen gen
+  le_maxGen := by
+    have := setVar_le_maxGen τ l.index (PSCell.mkEmptyCell.setLit l gen)
+    rwa [PSCell.setLit_generation PSCell.mkEmptyCell l gen] at this
+}
+
+def setVarToLit (τ : PS) (v : IVar) (l : ILit) : PS := { τ with
+  assignment := τ.assignment.setF v.index (PSCell.mkEmptyCell.setLit l τ.generation) PSCell.mkEmptyCell
+  maxGen := max τ.maxGen τ.generation
+  le_maxGen := by
+    have := setVar_le_maxGen τ v.index (PSCell.mkEmptyCell.setLit l τ.generation)
+    rwa [PSCell.setLit_generation PSCell.mkEmptyCell l τ.generation] at this
+}
+
+def setVarToLitUntil (τ : PS) (v : IVar) (l : ILit) (gen : Nat) : PS := { τ with
+  assignment := τ.assignment.setF v.index (PSCell.mkEmptyCell.setLit l gen) PSCell.mkEmptyCell
+  maxGen := max τ.maxGen gen
+  le_maxGen := by
+    have := setVar_le_maxGen τ v.index (PSCell.mkEmptyCell.setLit l gen)
+    rwa [PSCell.setLit_generation PSCell.mkEmptyCell l gen] at this
+}
+
+@[simp, inline] def setLitToLit (τ : PS) (l l_target : ILit) : PS :=
+  if polarity l then
+    τ.setVarToLit (toVar l) l_target
+  else
+    τ.setVarToLit (toVar l) (-l_target)
+
+@[simp, inline] def setLitToLitUntil (τ : PS) (l l_target : ILit) (gen : Nat) : PS :=
+  if polarity l then
+    τ.setVarToLitUntil (toVar l) l_target gen
+  else
+    τ.setVarToLitUntil (toVar l) (-l_target) gen
+
+def setVars (σ : PS) (L : List (IVar × ILit)) : PS :=
+  L.foldl (init := σ) (fun σ ⟨v, l⟩ => σ.setVarToLit v l)
+
+def setVars' (σ : PS) (A : Array (IVar × ILit)) : PS :=
+  A.foldl (init := σ) (fun σ ⟨v, l⟩ => σ.setVarToLit v l)
+
+def setVarsUntil (σ : PS) (L : List (IVar × ILit)) (gen : Nat) : PS :=
+  L.foldl (init := σ) (fun σ ⟨v, l⟩ => σ.setVarToLitUntil v l gen)
+
+def setVarsUntil' (σ : PS) (A : Array (IVar × ILit)) (gen : Nat) : PS :=
+  A.foldl (init := σ) (fun σ ⟨v, l⟩ => σ.setVarToLitUntil v l gen)
+
+theorem setVars_eq_setVars' {L : List (IVar × ILit)} {A : Array (IVar × ILit)} :
+  L = A.data → ∀ (σ : PS), σ.setVars L = σ.setVars' A := by sorry
+
+/- Lemmas -/
+
+@[simp] theorem setLit_size (τ : PS) (l : ILit) : (τ.setLit l).size = max τ.size (l.index + 1) := by
+  simp [setLit, size]
+
+-- Cayden TODO: Figure out which things are @[simp] in def vs. @[simp] theorems.
+theorem litValue_setLit_pos (τ : PS) (l : ILit) : (τ.setLit l).litValue l = .tr := by
+  by_cases hpol : polarity l
+  <;> by_cases hl : l.index < τ.size
+  <;> simp [litValue, varValue, size, setLit, PSCell.setLit, PSCell.setToTrue, PSCell.setToFalse,
+        hpol, hl, PSCell.varValue?, PSVal.negate, Array.getElem_setF]
+
+theorem litValue_setLit_neg (τ : PS) {l₁ l₂ : ILit} :
+    l₁ ≠ l₂ → (τ.setLit l₁).litValue l₂ = τ.litValue l₂ := by
+  intro hne
+  by_cases hpol₁ : polarity l₁
+  · by_cases hpol₂ : polarity l₂
+    · simp [hpol₁, hpol₂, litValue]
+      sorry
+    sorry
+  /-by_cases hpol : polarity l₂
+  · simp [litValue, hpol, setLit, Array.size_setF, -Array.get_eq_getElem]
+    by_cases hl₂ : l₂.index < τ.size
+    · rw [size] at hl₂
+      have : l₂.index < τ.assignment.size ∨ l₂.index < l₁.index + 1 := Or.inl hl₂
+      simp [hl₂, this, -Array.get_eq_getElem]
+      by_cases hpol₁ : polarity l₁
+      · rw [Array.getElem_setF' τ.assignment l₁.index ⟨τ.generation, PSVal.tr⟩ PSCell.mkEmptyCell]
+
+      done
+    done
+  --by_cases hpol : polarity l₂
+  --<;> by_cases hl₂ : l₂.index < τ.size
+  --<;> simp [litValue, setLit, hpol,
+  --    hl₂, Or.inl hl₂, Array.size_setF, PSCell.varValue?, PSVal.negate] -/
+  sorry
+  done
+
+/-! # New -/
+
+--ofFn (fun (idx : Fin maxVar) => PSCell.mkCell idx 0)
+
+/-- Initialize to an empty partial assignment,
+supporting variables in the range `[1, maxVar]`.
+
+The assignment will resize dynamically if it's used with
+a variable above the initial `maxVar`. -/
+
+def new (n : Nat) : PS where
+  assignment := Array.mkArray n PSCell.mkEmptyCell
+  generation := ⟨1, Nat.one_pos⟩
+  maxGen := 0
+  le_maxGen := by simp_all [List.mem_replicate]
+
+/-
+theorem new_WF (n : Nat) : (new n).WF := by
+  simp [new]
+  constructor
+  · intro i
+    sorry
+  · simp only [gt_iff_lt, zero_lt_one] -/
+
+/-! # Reset -/
+
+/-- Reset the assignment to an empty one. -/
+def reset (τ : PS) : PS :=
+  { τ with
+    generation := ⟨τ.maxGen + 1, Nat.succ_pos _⟩ }
+
+/-! # Bump -/
+
+/-- Clear all temporary assignments at the current generation. -/
+def bump (τ : PS) : PS :=
+  { τ with generation := τ.generation + 1 }
+
+
+section monadic
+
+/-! # Unit propagation -/
+
+/-
+
+Cayden note 1/8: In SR checking, the substitution witness σ is provided in the proof line,
+  and then never modified. Instead, a partial assignment α is produced and modified.
+
+To save memory and time, the substitution and partial assignments use the "generation bumping" strategy
+to clear out their computations after each proof line/group of hints.
+
+Since unit propagation is never done/evaluated against a substitution, proving its correctness is moot.
+But! We do need to compute a clause's reduction under a substitution, and so we need a theory for that.
+We also need to think about an efficient way to either compute a reduction OR make reduction and evaluation
+against a partial assignment happen in the same step (possibly using another "PPA" structure off to the side
+to record which literals have been seen in the reduction, so a tautology can be detected)
+
+-/
+
+inductive UPResult where
+  | falsified
+  | satisfied
+  | unit (l : ILit) (τ : PS) -- Updated substitution and unit literal l
+  | multipleUnassignedLiterals
+
+inductive UPDone where
+  | satisfied
+  | multipleUnassignedLiterals
+
+abbrev UPBox := ResultT UPDone (Option ILit)
+
+open ResultT UPResult UPDone PPA
+
+def sevalUP (σ : PS) (unit? : Option ILit) (l : ILit) : UPBox :=
+  match σ.litValue l with
+  | .tr => done .satisfied
+  | .fls => ok unit?
+  | .lit lit =>
+    match unit? with
+    | none => ok lit
+    | some u =>
+      if u = lit then ok unit?
+      -- Since σ is a substitution, tautology could occur
+      else if u = -lit then done .satisfied
+      else done .multipleUnassignedLiterals
+
+def foldUP (σ : PS) (C : IClause) := C.foldlM (sevalUP σ) none
+
+def unitProp (σ : PS) (C : IClause) : UPResult :=
+  match foldUP σ C with
+  | ok none => .falsified
+  | ok (some lit) => .unit lit (σ.setLit lit)
+  | done .satisfied => .satisfied
+  | done .multipleUnassignedLiterals => .multipleUnassignedLiterals
+
+def UP_motive_fn (σ : PS) (C : IClause) : ℕ → Option ILit → Prop
+  | idx, none => ∀ ⦃i : Fin C.size⦄, i < idx → σ.litValue C[i] = .fls
+  | idx, some lit => ∃ (i : Fin C.size), i < idx ∧ σ.litValue C[i] = .lit lit ∧
+      (∀ ⦃j : Fin C.size⦄, j < idx → j ≠ i → (σ.litValue C[j] = .fls ∨ σ.litValue C[j] = .lit lit))
+
+theorem SatisfiesM_UP (σ : PS) (C : IClause) :
+    SatisfiesM (fun
+      | none => ∀ l ∈ C.data, σ.litValue l = .fls
+      | some lit => ∃ (l : ILit), l ∈ C.data ∧ σ.litValue l = .lit lit ∧
+          (∀ l' ∈ C.data, l' ≠ l → (σ.litValue l' = .fls ∨ σ.litValue l' = .lit lit))) (foldUP σ C) := by
+  have := C.SatisfiesM_foldlM (init := (none : Option ILit)) (f := sevalUP σ)
+    (motive := UP_motive_fn σ C)
+    (h0 := by simp [UP_motive_fn])
+    (hf := by
+      unfold UP_motive_fn
+      simp only [SatisfiesM_ResultT_eq, getElem_fin]
+      -- Cayden question: is the proof more compact if I use pattern-matching with intro?
+      intro i box ih
+      intro
+      | none, hbox =>
+        intro j hj
+        unfold sevalUP at hbox
+        match hσ : σ.litValue C[i.val] with
+        | .tr => simp_rw [hσ] at hbox
+        | .fls =>
+          simp_rw [hσ, ok.injEq] at hbox; subst hbox
+          rcases Order.lt_succ_iff_eq_or_lt.mp hj with (hj | hj)
+          · rw [Fin.ext hj]; exact hσ
+          · exact ih hj
+        | .lit lit =>
+          simp [hσ] at hbox
+          match box with
+          | none => simp at hbox
+          | some u =>
+            rcases eq_trichotomy u lit with (rfl | rfl | hvar)
+            · simp at hbox
+            · simp at hbox
+            · simp [ne_of_var_ne hvar, ne_of_var_ne ((toVar_negate lit).symm ▸ hvar)] at hbox
+      | some u, hbox =>
+        rename ILit => lit
+        unfold sevalUP at hbox
+        match hσ : σ.litValue C[i.val] with
+        | .tr => simp_rw [hσ] at hbox
+        | .fls =>
+          simp_rw [hσ, ok.injEq] at hbox; subst hbox
+          rcases ih with ⟨idx, hidx_lt, hidxσ, hidx_fls⟩
+          use idx, lt_succ_of_lt hidx_lt, hidxσ
+          intro j hj
+          rcases lt_or_eq_of_le (le_of_lt_succ hj) with (h | h)
+          · exact hidx_fls h
+          · replace h := Fin.ext h; subst h; intro _; exact Or.inl hσ
+        | .lit lit' =>
+          simp [hσ] at hbox
+          match box with
+          | none =>
+            simp at hbox; subst hbox
+            have : C[i.val] ∈ C.data := Array.getElem_mem_data C i.isLt
+            use i, lt_succ_self _, hσ
+            intro j hj
+            rcases lt_or_eq_of_le (le_of_lt_succ hj) with (h | h)
+            · intro _; exact Or.inl (ih h)
+            · replace h := Fin.ext h; subst h; intro hcon; contradiction
+          | some u =>
+            rcases eq_trichotomy u lit' with (rfl | rfl | hvar)
+            · simp at hbox; subst hbox
+              rcases ih with ⟨idx, hidx_lt, hidxσ, hidx_fls⟩
+              use idx, lt_succ_of_lt hidx_lt, hidxσ
+              intro j hj
+              rcases lt_or_eq_of_le (le_of_lt_succ hj) with (h | h)
+              · exact hidx_fls h
+              · replace h := Fin.ext h; subst h; intro _; exact Or.inr hσ
+            · simp at hbox
+            · simp [ne_of_var_ne hvar, ne_of_var_ne ((toVar_negate lit').symm ▸ hvar)] at hbox)
+  apply SatisfiesM.imp this
+  intro
+  | none =>
+    intro h l hl
+    rcases Array.mem_data_iff.mp hl with ⟨i, rfl⟩
+    exact h i.isLt
+  | some lit =>
+    simp [UP_motive_fn]
+    intro i hi ih
+    use C[i.val], Array.getElem_mem_data C i.isLt, hi
+    intro l hl₁ hl₂
+    rcases Array.mem_data_iff.mp hl₁ with ⟨j, rfl⟩
+    apply ih
+    exact ne_of_apply_ne (C[·]) hl₂
+
+theorem contradiction_of_UP_falsified {σ : PS} {C : IClause} :
+    σ.unitProp C = .falsified → (C.toPropFun).bind σ.toSubst ≤ ⊥ := by
+  unfold unitProp
+  intro h_falsified
+  split at h_falsified <;> try simp at h_falsified
+  clear h_falsified
+  rename (foldUP σ C = ok none) => h
+  refine entails_ext.mpr fun τ hτ => ?_
+  rw [satisfies_bind] at hτ
+  have ⟨lit, hlit, hτlit⟩ := Clause.satisfies_iff.mp hτ
+  have := SatisfiesM_ResultT_eq.mp (SatisfiesM_UP σ C) none h lit hlit
+  clear h hτ
+  replace hτlit := satisfies_iff.mp hτlit
+  cases hpol : polarity lit
+  <;> simp [hpol, PropAssignment.preimage] at hτlit
+  · rw [litValue_eq_varValue_neg hpol, PSVal.negate_rhs_eq_lhs_negate, PSVal.negate,
+          varValue_tr_iff, bind_distrib] at this
+    rw [this] at hτlit
+    contradiction
+  · rw [litValue_eq_varValue_pos hpol, varValue_fls_iff, bind_distrib] at this
+    rw [this] at hτlit
+    exact hτlit
+
+theorem extended_of_UP_unit {σ σ' : PS} {C : IClause} {l : ILit} :
+    σ.unitProp C = .unit l σ' →
+      (C.toPropFun).bind σ.toSubst ≤ l.toPropFun ∧
+      (∃ lit ∈ C.data, σ.litValue lit = .lit l ∧ σ'.litValue l = .tr) := by
+      -- Cayden question: how to express this in an abstract way? Perhaps with a bind (l.bind σ) or as a (. ∘ .) of two subs
+  unfold unitProp
+  intro h_unit
+  split at h_unit <;> try simp at h_unit
+  --clear h_unit
+  rename ILit => lit
+  rename (foldUP σ C = ok (some lit)) => h
+  rcases h_unit with ⟨rfl, rfl⟩
+  have hlv := SatisfiesM_ResultT_eq.mp (SatisfiesM_UP σ C) (some lit) h
+  clear h
+  rcases hlv with ⟨l, hl_mem, hσl, ih⟩
+  constructor
+  · refine entails_ext.mpr fun τ hτ => ?_
+    rw [satisfies_bind] at hτ
+    by_cases heq : l = lit
+    · subst heq
+      rw [Clause.satisfies_iff] at hτ; rcases hτ with ⟨l', hl'_mem, hl'⟩
+      rw [← satisfies_bind] at hl'
+      sorry -- Proof got stuck here. And we may not need unit propagaion after all
+      done
+    · sorry
+      done
+    done
+  · exact ⟨l, hl_mem, hσl, litValue_setLit_pos _ _⟩
+  done
+
+-- We have to carry along a PPA to store the unset literals and check for tautologies (Cayden later comment: why??)
+
+/-! # Reduction -/
+
+-- We do something very similar to "unit propagation", except we don't modify σ
+
+inductive ReductionResult where
+  | falsified
+  | satisfied
+  | reduced
+  | notReduced
+
+abbrev RedBox := ResultT PPA (PPA × Bool × Bool)
+
+open ResultT ReductionResult
+
+def sevalRed (σ : PS) (p : PPA × Bool × Bool) (l : ILit) : RedBox :=
+  let ⟨τ, reduced?, unassigned?⟩ := p
+  match σ.litValue l with
+  | .tr => done τ
+  | .fls => ok ⟨τ, true, unassigned?⟩
+  | .lit lit =>
+    match τ.litValue? lit with
+    | none => ok ⟨τ.setLit lit, reduced? || (l != lit), true⟩
+    | some true => ok ⟨τ, reduced? || (l != lit), true⟩
+    | some false => done τ
+
+def foldRed (σ : PS) (τ : PPA) (C : IClause) := C.foldlM (sevalRed σ) ⟨τ.reset, false, false⟩
+
+def reduced? (σ : PS) (τ : PPA) (C : IClause) : ReductionResult × PPA :=
+  match foldRed σ τ C with
+  | ok ⟨τ, true, false⟩  => (.falsified, τ)
+  | ok ⟨τ, true, true⟩   => (.reduced, τ)
+  | ok ⟨τ, false, true⟩  => (.notReduced, τ)
+  | ok ⟨τ, false, false⟩ => (.notReduced, τ) -- Shouldn't get this case, except if C is empty
+  | done τ => (.satisfied, τ)
+
+theorem reduced?_satisfied_iff {σ : PS} {τ τ' : PPA} {C : IClause} :
+    σ.reduced? τ C = (.satisfied, τ') ↔ (C.toPropFun).bind σ.toSubst = ⊤ := by
+  sorry
+  done
+
+theorem reduced?_falsified_iff {σ : PS} {τ τ' : PPA} {C : IClause} :
+    σ.reduced? τ C = (.falsified, τ') ↔ (C.toPropFun).bind σ.toSubst ≤ ⊥ := by
+  sorry
+  done
+
+theorem reduced?_notReduced_iff {σ : PS} {τ τ' : PPA} {C : IClause} :
+    σ.reduced? τ C = (.notReduced, τ') ↔ (C.toPropFun).bind σ.toSubst = ↑C := by
+  sorry
+  done
+
+theorem reduced?_reduced {σ : PS} {τ τ' : PPA} {C : IClause} :
+    σ.reduced? τ C = (.reduced, τ') →
+      ((C.toPropFun).bind σ.toSubst ≠ ⊤ ∧ (C.toPropFun).bind σ.toSubst ≠ ⊥) := by
+  sorry
+  done
+
+/- Reduction without tautology checking -/
+
+def seval (σ : PS) (p : Bool × Bool) (l : ILit) : ResultT Unit (Bool × Bool) :=
+  -- Has there been a non-id map, and has there been an literal that's unassigned
+  let ⟨reduced?, unassigned?⟩ := p
+  match σ.litValue l with
+  | .tr => done ()
+  | .fls => ok (true, unassigned?)
+  | .lit lit => ok (reduced? || (l != lit), true)
+
+def reduce (σ : PS) (C : IClause) : ReductionResult :=
+  match C.foldlM (seval σ) (false, false) with
+  | ok (true, true) => .reduced
+  | ok (true, false) => .falsified
+  | ok (false, true) => .notReduced
+  | ok (false, false) => .notReduced -- Shouldn't get this, unless if C is empty
+  | done () => .satisfied
+
+-- TODO: It is possible only the forward directions are needed
+theorem reduce_satisfied_iff {σ : PS} {C : IClause} :
+    σ.reduce C = .satisfied ↔ (C.toPropFun).bind σ.toSubst = ⊤ := by
+  sorry
+  done
+
+theorem reduce_falsified_iff {σ : PS} {C : IClause} :
+    σ.reduce C = .falsified ↔ (C.toPropFun).bind σ.toSubst ≤ ⊥ := by
+  sorry
+  done
+
+theorem reduce_notReduced_iff {σ : PS} {C : IClause} :
+    σ.reduce C = .notReduced ↔ (C.toPropFun).bind σ.toSubst = ↑C := by
+  sorry
+  done
+
+theorem reduce_reduced {σ : PS} {C : IClause} :
+    σ.reduce C = .reduced ↔
+      ((C.toPropFun).bind σ.toSubst ≠ ⊤ ∧ (C.toPropFun).bind σ.toSubst ≠ ⊥) := by
+  sorry
+  done
+
+end monadic /- section -/
+
+end Trestle.PS
